bunch of low level stuff

src/computational_monads/simulation_semantics/constructions/logging/query_log/basic.lean
@@ -61,115 +61,60 @@ dite_eq_iff.2 (or.inr ⟨hi, rfl⟩)
 
 end log_query
 
-section lookup
+
+section not_queried
 
 variable [spec.computable]
 
-/-- Find the query output of the first oracle query with the given input.
-  Result is returned as an `option`, with `none` for inputs that haven't previously been queried.
-  Main use case is for using the log as a cache for repeated queries. -/
-def lookup (log : query_log spec) (i : spec.ι) (t : spec.domain i) :
-  option (spec.range i) :=
-((log i).find $ (= t) ∘ prod.fst).map prod.snd
+-- Check that a input was never queried
+def not_queried (log : query_log spec) (i : spec.ι) (t : spec.domain i) : bool :=
+((log i).find ((=) t ∘ prod.fst)).is_none
 
-@[simp]
-lemma lookup_init (spec : oracle_spec) [spec.computable]
-  (i : spec.ι) (t : spec.domain i) :
-  (init spec).lookup i t = none :=
-option.map_none'
-
-/-- Most general version of the lemma is somewhat cumbersome because of the equality induction.
-  More specific versions given below are usually more usefull -/
-lemma lookup_log_query (i j : spec.ι)
-  (t : spec.domain i) (t' : spec.domain j) (u : spec.range i) :
-  (log.log_query i t u).lookup j t' = if hi : i = j
-    then (if hi.rec_on t = t' then hi.rec_on (some u) else log.lookup j t') else log.lookup j t' := 
-begin
-  split_ifs with hi ht,
-  { induction hi, induction ht,
-    simp only [lookup, log_query_apply_same_index,
-      list.find_cons_of_pos, function.comp_app, option.map_some'] },
-  { induction hi,
-    refine congr_arg (option.map prod.snd) _,
-    refine (log.log_query_apply_same_index i t u).symm ▸ _,
-    exact list.find_cons_of_neg (log i) ht },
-  { refine congr_arg (option.map prod.snd ∘ _) _,
-    exact (log.log_query_apply_of_index_ne hi t u) }
-end
-
-@[simp]
-lemma lookup_log_query_same_index (i : spec.ι)
-  (t t' : spec.domain i) (u : spec.range i) :
-  (log.log_query i t u).lookup i t' = if t = t' then some u else log.lookup i t' :=
-trans (log.lookup_log_query  i i t t' u) (dif_pos rfl)
-
-lemma lookup_log_query_of_index_ne (i j : spec.ι) (hi : i ≠ j)
-  (t : spec.domain i) (t' : spec.domain j) (u : spec.range i) :
-  (log.log_query i t u).lookup j t' = log.lookup j t' :=
-trans (log.lookup_log_query i j t t' u) (dif_neg hi)
-
-@[simp]
-lemma lookup_log_query_same_input (i : spec.ι)
-  (t : spec.domain i) (u : spec.range i) :
-  (log.log_query i t u).lookup i t = some u :=
-trans (log.lookup_log_query_same_index i t t u) (if_pos rfl)
-
-lemma lookup_log_query_of_input_ne (i : spec.ι)
-  (t t' : spec.domain i) (ht : t ≠ t') (u : spec.range i) :
-  (log.log_query i t u).lookup i t' = log.lookup i t' :=
-trans (log.lookup_log_query_same_index i t t' u) (if_neg ht)
-
-end lookup
-
-section lookup_fst
-
-variable [spec.computable]
-
-/-- `lookup`, but only checking the front element of the list.
-  Main use case is using the `query_log` is a seed for a second computation -/
-def lookup_fst (log : query_log spec) (i : spec.ι) (t : spec.domain i) :
-  option (spec.range i) :=
-match log i with
-| [] := none
-| ((t', u)) :: _ := if t = t' then some u else none
-end
-
-lemma lookup_fst_init (spec : oracle_spec) [spec.computable]
-  (i : spec.ι) (t : spec.domain i) :
-  (query_log.init spec).lookup_fst i t = none :=
+lemma not_queried_def (i : spec.ι) (t : spec.domain i) :
+  log.not_queried i t = ((log i).find ((=) t ∘ prod.fst)).is_none :=
 rfl
 
-lemma lookup_fst_log_query (i j : spec.ι)
+lemma not_queried_init_eq_tt (spec : oracle_spec) [spec.computable]
+  (i : spec.ι) (t : spec.domain i) :
+  (init spec).not_queried i t = tt :=
+rfl
+
+lemma not_queried_log_query (i j : spec.ι)
   (t : spec.domain i) (t' : spec.domain j) (u : spec.range i) :
-  (log.log_query i t u).lookup_fst j t' = if hi : i = j
-    then (if hi.rec_on t = t' then hi.rec_on (some u) else none) else log.lookup_fst j t' :=
+  (log.log_query i t u).not_queried j t' =
+    (log.not_queried j t') && (if hi : i = j then (hi.rec_on t ≠ t') else tt) :=
 begin
-  split_ifs with hi ht,
-  { induction hi, induction ht,
-    simp only [lookup_fst, log_query_apply_same_index, eq_self_iff_true, if_true] },
+  split_ifs with hi,
   { induction hi,
-    simpa [lookup_fst] using ne.symm ht },
-  { simp only [lookup_fst, log_query_apply_of_index_ne _ hi] }
+    rw [not_queried, log_query_apply_same_index],
+    by_cases ht : t' = t,
+    { induction ht,
+      have : (eq t' ∘ prod.fst) (t', u) := (function.comp_app (eq t') prod.fst (t', u)).symm ▸ rfl,
+      simp only [list.find_cons_of_pos _ this, option.is_none_some, ne.def, eq_self_iff_true,
+        not_true, to_bool_false_eq_ff, band_ff] },
+    { have : ¬ (eq t' ∘ prod.fst) (t, u) := by simp only [ht, function.comp_app, not_false_iff],
+      simpa only [list.find_cons_of_neg _ this, ht, ne.symm ht,
+        ne.def, not_false_iff, to_bool_true_eq_tt, band_tt] } },
+  { simp only [not_queried, log_query_apply_of_index_ne log hi, band_tt] }
 end
 
-lemma lookup_fst_log_query_of_index_eq {i j : spec.ι} (hi : i = j)
+lemma not_queried_log_query_of_index_eq {i j : spec.ι} (hi : i = j)
   (t : spec.domain i) (t' : spec.domain j) (u : spec.range i) :
-  (log.log_query i t u).lookup_fst j t' =
-    if hi.rec_on t = t' then hi.rec_on (some u) else none :=
-(log.lookup_fst_log_query i j t t' u).trans (dif_pos hi)
+  (log.log_query i t u).not_queried j t' = (log.not_queried j t') && (hi.rec_on t ≠ t') :=
+(log.not_queried_log_query i j t t' u).trans (congr_arg ((&&) $ log.not_queried j t') (dif_pos hi))
 
-lemma lookup_fst_log_query_same_index (i : spec.ι)
+lemma not_queried_log_query_same_index (i : spec.ι)
   (t t' : spec.domain i) (u : spec.range i) :
-  (log.log_query i t u).lookup_fst i t' =
-    if t = t' then some u else none :=
-log.lookup_fst_log_query_of_index_eq rfl t t' u
+  (log.log_query i t u).not_queried i t' = (log.not_queried i t') && (t ≠ t') :=
+log.not_queried_log_query_of_index_eq rfl t t' u
 
-lemma lookup_fst_log_query_of_index_ne {i j : spec.ι} (hi : i ≠ j)
+lemma not_queried_log_query_of_index_ne {i j : spec.ι} (hi : i ≠ j)
   (t : spec.domain i) (t' : spec.domain j) (u : spec.range i) :
-  (log.log_query i t u).lookup_fst j t' = log.lookup_fst j t' :=
-(log.lookup_fst_log_query i j t t' u).trans (dif_neg hi)
+  (log.log_query i t u).not_queried j t' = log.not_queried j t' :=
+(log.not_queried_log_query i j t t' u).trans 
+  ((congr_arg _ (dif_neg hi)).trans (band_tt _))
 
-end lookup_fst
+end not_queried
 
 section map_at_index
 
@@ -231,7 +176,6 @@ end
 
 end map_at_index
 
-
 section drop_at_index
 
 def drop_at_index [spec.computable] (log : query_log spec)
@@ -292,19 +236,6 @@ begin
 end
 
 end drop_at_index
-
-section get_index
-
-/-- Get the index of the first query with the given input `t`.
-  Returns `none` if the input has never been queried
-  TODO: check if the fold should be right or left
-  TODO: `not_queried` can be defined using this instead? -/
-def index_of_input [spec.computable] (log : query_log spec)
-  (i : spec.ι) (t : spec.domain i) : option ℕ :=
-(log i).foldr_with_index
-  (λ n ⟨t', _⟩ m, if t' = t then some n else m) none
-
-end get_index
 
 section remove_head
 
@@ -376,121 +307,5 @@ lemma remove_head_log_query_of_index_ne {i j : spec.ι} (hi : i ≠ j)
 trans (log.remove_head_log_query i j t u) (if_neg hi)
 
 end remove_head
-
-section not_queried
-
-variable [spec.computable]
-
--- Check that a input was never queried
-def not_queried (log : query_log spec) (i : spec.ι) (t : spec.domain i) : bool :=
-((log i).find ((=) t ∘ prod.fst)).is_none
-
-lemma not_queried_def (i : spec.ι) (t : spec.domain i) :
-  log.not_queried i t = ((log i).find ((=) t ∘ prod.fst)).is_none :=
-rfl
-
-lemma not_queried_init_eq_tt (spec : oracle_spec) [spec.computable]
-  (i : spec.ι) (t : spec.domain i) :
-  (init spec).not_queried i t = tt :=
-rfl
-
-lemma not_queried_log_query (i j : spec.ι)
-  (t : spec.domain i) (t' : spec.domain j) (u : spec.range i) :
-  (log.log_query i t u).not_queried j t' =
-    (log.not_queried j t') && (if hi : i = j then (hi.rec_on t ≠ t') else tt) :=
-begin
-  split_ifs with hi,
-  { induction hi,
-    rw [not_queried, log_query_apply_same_index],
-    by_cases ht : t' = t,
-    { induction ht,
-      have : (eq t' ∘ prod.fst) (t', u) := (function.comp_app (eq t') prod.fst (t', u)).symm ▸ rfl,
-      simp only [list.find_cons_of_pos _ this, option.is_none_some, ne.def, eq_self_iff_true,
-        not_true, to_bool_false_eq_ff, band_ff] },
-    { have : ¬ (eq t' ∘ prod.fst) (t, u) := by simp only [ht, function.comp_app, not_false_iff],
-      simpa only [list.find_cons_of_neg _ this, ht, ne.symm ht,
-        ne.def, not_false_iff, to_bool_true_eq_tt, band_tt] } },
-  { simp only [not_queried, log_query_apply_of_index_ne log hi, band_tt] }
-end
-
-lemma not_queried_log_query_of_index_eq {i j : spec.ι} (hi : i = j)
-  (t : spec.domain i) (t' : spec.domain j) (u : spec.range i) :
-  (log.log_query i t u).not_queried j t' = (log.not_queried j t') && (hi.rec_on t ≠ t') :=
-(log.not_queried_log_query i j t t' u).trans (congr_arg ((&&) $ log.not_queried j t') (dif_pos hi))
-
-lemma not_queried_log_query_same_index (i : spec.ι)
-  (t t' : spec.domain i) (u : spec.range i) :
-  (log.log_query i t u).not_queried i t' = (log.not_queried i t') && (t ≠ t') :=
-log.not_queried_log_query_of_index_eq rfl t t' u
-
-lemma not_queried_log_query_of_index_ne {i j : spec.ι} (hi : i ≠ j)
-  (t : spec.domain i) (t' : spec.domain j) (u : spec.range i) :
-  (log.log_query i t u).not_queried j t' = log.not_queried j t' :=
-(log.not_queried_log_query i j t t' u).trans 
-  ((congr_arg _ (dif_neg hi)).trans (band_tt _))
-
-end not_queried
-
-section to_seed
-
-/-- Wrapping function that just reverses every list in the given `query_log`. 
-  Intended to turn a log into something that can be used as a seed for a computation.
-  Needed because the logging function adds the new queries to the front of the list  -/
-def to_seed (log : query_log spec) :
-  query_log spec :=
-λ i, (log i).reverse
-
-@[simp]
-lemma to_seed_apply (log : query_log spec) (i : spec.ι) :
-  log.to_seed i = (log i).reverse :=
-rfl
-
-@[simp]
-lemma to_seed_init (spec : oracle_spec) :
-  (init spec).to_seed = init spec :=
-rfl
-
-lemma to_seed_log_query [spec.computable] (log : query_log spec)
-  (i : spec.ι) (t : spec.domain i) (u : spec.range i) :
-  (log.log_query i t u).to_seed = λ j, if hi : i = j
-    then log.to_seed j ++ [hi.rec_on (t, u)] else log.to_seed j :=
-begin
-  refine ext (λ j, _),
-  split_ifs,
-  { induction h,
-    exact trans (congr_arg list.reverse $ log.log_query_apply_same_index i t u)
-      (list.reverse_cons (t, u) (log i)) },
-  { exact congr_arg list.reverse (log.log_query_apply_of_index_ne h t u) }
-end
-
-end to_seed
-
--- Different lookup that only looks at head, and removes the element from the cache
-def take_fst [spec.computable]
-  (log : query_log spec) (i : spec.ι) (t : spec.domain i) :
-  option (spec.range i) × query_log spec :=
-match (log i).nth 0 with
-| none := (none, query_log.init spec)
-| some ⟨t', u⟩ := if t' = t then (some u, log.remove_head i)
-    else (none, query_log.init spec) -- TODO: maybe don't clear everything here?
-end
-
-/-- Remove parts of the cache after the query chosen to fork on -/
-def fork_cache [spec.computable] (log : query_log spec)
-  (i : spec.ι) (n : option ℕ) : query_log spec :=
-match n with
-| none := log -- TODO: this case doesn't really matter but whatever
-| (some m) := log.drop_at_index i m
-end
-
-def query_input_same_at (cache cache' : query_log spec)
-  (i : spec.ι) (n : ℕ) : Prop :=
-((cache i).nth n).map prod.fst = ((cache i).nth n).map prod.fst
-
--- query_results are different for the two caches at `n`
-def query_output_diff_at (cache cache' : query_log spec)
-  (i : spec.ι) (n : ℕ) : Prop :=
-((cache i).nth n).map prod.snd ≠ ((cache' i).nth n).map prod.snd
-
 
 end query_log
