src/computational_monads/simulation_semantics/constructions/identity_oracle.lean
@@ -1,0 +1,86 @@
+import computational_monads.simulation_semantics.constructions.stateless_oracle
+
+open oracle_comp oracle_spec
+
+variables {A B : Type} {spec spec' spec'' : oracle_spec}
+  (oa : oracle_comp spec A)
+
+def identity_oracle (spec : oracle_spec) : simulation_oracle spec spec :=
+⟪ query ⟫
+
+notation `idₛ` := identity_oracle _
+
+@[simp]
+lemma default_state_identity_oracle :
+  (identity_oracle spec).default_state = () := rfl
+
+@[simp]
+lemma identity_oracle_apply (i : spec.ι) (t : spec.domain i) (s : unit) :
+  (identity_oracle spec).o i (t, s) = query i t >>= λ u, return (u, ()) := rfl
+
+section simulate
+
+
+@[simp]
+lemma eval_distribution_simulate_identity_oracle [spec.finite_range] 
+  (oa : oracle_comp spec A) (s : unit) :
+  ⟦simulate idₛ oa s⟧ = (λ a, (a, ())) <$> ⟦oa⟧ :=
+begin
+  induction oa,
+  {
+    simp,
+    sorry
+  },
+  sorry, sorry
+end
+
+@[simp]
+lemma support_simulate_identity_oracle_pure (a : A) (s : unit) :
+  (simulate idₛ (pure a : oracle_comp spec A) s).support = {(a, ())} :=
+support_simulate_stateless_oracle_pure _ a s
+
+@[simp]
+lemma support_simulate_identity_oracle (oa : oracle_comp spec A) (s : unit) :
+  (simulate idₛ oa s).support = {x | x.1 ∈ oa.support} :=
+begin
+  induction oa with A a A B oa ob hoa hob i t,
+  {
+    ext x,
+    simp [prod.eq_iff_fst_eq_snd_eq, punit_eq x.snd s],
+  },
+  {
+    ext x,
+    simp [hoa, hob],
+    sorry,
+  },
+  {
+    ext x,
+    induction x with x_fst x_snd,
+    simp,
+    refine punit_eq () x_snd,
+  }
+end
+
+lemma mem_support_simulate_identity_oracle_iff (oa : oracle_comp spec A) (s : unit) (x : A × unit) :
+  x ∈ (simulate idₛ oa s).support ↔ x.1 ∈ oa.support :=
+begin
+  simp,
+  refine iff.rfl,
+end
+
+end simulate
+
+section simulate'
+
+@[simp]
+lemma support_simulate'_identity_oracle (oa : oracle_comp spec A) (s : unit) :
+  (simulate' idₛ oa s).support = oa.support :=
+begin
+  rw [support_simulate', support_simulate_identity_oracle],
+  ext x,
+  simp only [set.mem_image, set.mem_set_of_eq,
+    prod.exists, exists_and_distrib_right, exists_eq_right],
+  refine ⟨λ h, h.rec_on (λ _ h, h), λ h, ⟨(), h⟩⟩,
+end
+
+end simulate'
