src/computational_monads/simulation_semantics/constructions/logging/caching_oracle.lean
@@ -1,5 +1,6 @@
 import computational_monads.simulation_semantics.constructions.logging.logging_oracle
 import computational_monads.simulation_semantics.oracle_compose
+import computational_monads.simulation_semantics.constructions.uniform_oracle
 
 open oracle_comp oracle_spec
 
