src/computational_monads/simulation_semantics/constructions/logging/query_log/fork.lean
@@ -1,0 +1,64 @@
+import computational_monads.simulation_semantics.constructions.logging.query_log.basic
+
+namespace query_log
+
+variables {spec : oracle_spec} (log : query_log spec)
+
+section fork_cache
+
+/-- Remove parts of the cache after the query chosen to fork on.
+  Just wraps a call to `drop_at_index`, dropping nothing if the input is `none` -/
+def fork_cache [spec.computable] (log : query_log spec)
+  (i : spec.ι) (n : option ℕ) : query_log spec :=
+match n with
+| none := log -- TODO: this case doesn't really matter but whatever
+| (some m) := log.drop_at_index i m
+end
+
+variable [spec.computable]
+
+lemma fork_cache_init (i : spec.ι) (n : option ℕ) :
+  (query_log.init spec).fork_cache i n = query_log.init spec :=
+begin
+  induction n with n,
+  { exact rfl },
+  { exact drop_at_index_init n i }
+end
+
+end fork_cache
+
+section to_seed
+
+/-- Wrapping function that just reverses every list in the given `query_log`. 
+  Intended to turn a log into something that can be used as a seed for a computation.
+  Needed because the logging function adds the new queries to the front of the list  -/
+def to_seed (log : query_log spec) :
+  query_log spec :=
+λ i, (log i).reverse
+
+@[simp]
+lemma to_seed_apply (log : query_log spec) (i : spec.ι) :
+  log.to_seed i = (log i).reverse :=
+rfl
+
+@[simp]
+lemma to_seed_init (spec : oracle_spec) :
+  (init spec).to_seed = init spec :=
+rfl
+
+lemma to_seed_log_query [spec.computable] (log : query_log spec)
+  (i : spec.ι) (t : spec.domain i) (u : spec.range i) :
+  (log.log_query i t u).to_seed = λ j, if hi : i = j
+    then log.to_seed j ++ [hi.rec_on (t, u)] else log.to_seed j :=
+begin
+  refine ext (λ j, _),
+  split_ifs,
+  { induction h,
+    exact trans (congr_arg list.reverse $ log.log_query_apply_same_index i t u)
+      (list.reverse_cons (t, u) (log i)) },
+  { exact congr_arg list.reverse (log.log_query_apply_of_index_ne h t u) }
+end
+
+end to_seed
+
+end query_log
