src/computational_monads/simulation_semantics/constructions/logging/query_log/lookup.lean
@@ -1,0 +1,144 @@
+import computational_monads.simulation_semantics.constructions.logging.query_log.basic
+
+namespace query_log
+
+variables {spec : oracle_spec} (log : query_log spec)
+variable [spec.computable]
+
+section lookup
+
+/-- Find the query output of the first oracle query with the given input.
+  Result is returned as an `option`, with `none` for inputs that haven't previously been queried.
+  Main use case is for using the log as a cache for repeated queries. -/
+def lookup (log : query_log spec) (i : spec.ι) (t : spec.domain i) :
+  option (spec.range i) :=
+((log i).find $ (= t) ∘ prod.fst).map prod.snd
+
+@[simp]
+lemma lookup_init (spec : oracle_spec) [spec.computable]
+  (i : spec.ι) (t : spec.domain i) :
+  (init spec).lookup i t = none :=
+option.map_none'
+
+/-- Most general version of the lemma is somewhat cumbersome because of the equality induction.
+  More specific versions given below are usually more usefull -/
+lemma lookup_log_query (i j : spec.ι)
+  (t : spec.domain i) (t' : spec.domain j) (u : spec.range i) :
+  (log.log_query i t u).lookup j t' = if hi : i = j
+    then (if hi.rec_on t = t' then hi.rec_on (some u) else log.lookup j t') else log.lookup j t' := 
+begin
+  split_ifs with hi ht,
+  { induction hi, induction ht,
+    simp only [lookup, log_query_apply_same_index,
+      list.find_cons_of_pos, function.comp_app, option.map_some'] },
+  { induction hi,
+    refine congr_arg (option.map prod.snd) _,
+    refine (log.log_query_apply_same_index i t u).symm ▸ _,
+    exact list.find_cons_of_neg (log i) ht },
+  { refine congr_arg (option.map prod.snd ∘ _) _,
+    exact (log.log_query_apply_of_index_ne hi t u) }
+end
+
+@[simp]
+lemma lookup_log_query_same_index (i : spec.ι)
+  (t t' : spec.domain i) (u : spec.range i) :
+  (log.log_query i t u).lookup i t' = if t = t' then some u else log.lookup i t' :=
+trans (log.lookup_log_query  i i t t' u) (dif_pos rfl)
+
+lemma lookup_log_query_of_index_ne (i j : spec.ι) (hi : i ≠ j)
+  (t : spec.domain i) (t' : spec.domain j) (u : spec.range i) :
+  (log.log_query i t u).lookup j t' = log.lookup j t' :=
+trans (log.lookup_log_query i j t t' u) (dif_neg hi)
+
+@[simp]
+lemma lookup_log_query_same_input (i : spec.ι)
+  (t : spec.domain i) (u : spec.range i) :
+  (log.log_query i t u).lookup i t = some u :=
+trans (log.lookup_log_query_same_index i t t u) (if_pos rfl)
+
+lemma lookup_log_query_of_input_ne (i : spec.ι)
+  (t t' : spec.domain i) (ht : t ≠ t') (u : spec.range i) :
+  (log.log_query i t u).lookup i t' = log.lookup i t' :=
+trans (log.lookup_log_query_same_index i t t' u) (if_neg ht)
+
+end lookup
+
+section lookup_fst
+
+/-- `lookup`, but only checking the front element of the list.
+  Main use case is using the `query_log` is a seed for a second computation -/
+def lookup_fst (log : query_log spec) (i : spec.ι) (t : spec.domain i) :
+  option (spec.range i) :=
+match log i with
+| [] := none
+| ((t', u)) :: _ := if t = t' then some u else none
+end
+
+lemma lookup_fst_init (spec : oracle_spec) [spec.computable]
+  (i : spec.ι) (t : spec.domain i) :
+  (query_log.init spec).lookup_fst i t = none :=
+rfl
+
+lemma lookup_fst_log_query (i j : spec.ι)
+  (t : spec.domain i) (t' : spec.domain j) (u : spec.range i) :
+  (log.log_query i t u).lookup_fst j t' = if hi : i = j
+    then (if hi.rec_on t = t' then hi.rec_on (some u) else none) else log.lookup_fst j t' :=
+begin
+  split_ifs with hi ht,
+  { induction hi, induction ht,
+    simp only [lookup_fst, log_query_apply_same_index, eq_self_iff_true, if_true] },
+  { induction hi,
+    simpa [lookup_fst] using ne.symm ht },
+  { simp only [lookup_fst, log_query_apply_of_index_ne _ hi] }
+end
+
+lemma lookup_fst_log_query_of_index_eq {i j : spec.ι} (hi : i = j)
+  (t : spec.domain i) (t' : spec.domain j) (u : spec.range i) :
+  (log.log_query i t u).lookup_fst j t' =
+    if hi.rec_on t = t' then hi.rec_on (some u) else none :=
+(log.lookup_fst_log_query i j t t' u).trans (dif_pos hi)
+
+lemma lookup_fst_log_query_same_index (i : spec.ι)
+  (t t' : spec.domain i) (u : spec.range i) :
+  (log.log_query i t u).lookup_fst i t' =
+    if t = t' then some u else none :=
+log.lookup_fst_log_query_of_index_eq rfl t t' u
+
+lemma lookup_fst_log_query_of_index_ne {i j : spec.ι} (hi : i ≠ j)
+  (t : spec.domain i) (t' : spec.domain j) (u : spec.range i) :
+  (log.log_query i t u).lookup_fst j t' = log.lookup_fst j t' :=
+(log.lookup_fst_log_query i j t t' u).trans (dif_neg hi)
+
+end lookup_fst
+
+section get_index
+
+/-- Get the index of the first query with the given input `t`.
+  Returns `none` if the input has never been queried
+  TODO: check if the fold should be right or left
+  TODO: `not_queried` can be defined using this instead? -/
+def get_index_of_input [spec.computable] (log : query_log spec)
+  (i : spec.ι) (t : spec.domain i) : option ℕ :=
+(log i).foldr_with_index
+  (λ n ⟨t', _⟩ m, if t' = t then some n else m) none
+
+end get_index
+
+section query_input_same_at
+
+def query_input_same_at (cache cache' : query_log spec)
+  (i : spec.ι) (n : ℕ) : Prop :=
+((cache i).nth n).map prod.fst = ((cache i).nth n).map prod.fst
+
+end query_input_same_at
+
+section query_input_diff_at
+
+-- query_results are different for the two caches at `n`
+def query_output_diff_at (cache cache' : query_log spec)
+  (i : spec.ι) (n : ℕ) : Prop :=
+((cache i).nth n).map prod.snd ≠ ((cache' i).nth n).map prod.snd
+
+end query_input_diff_at
+
+end query_log
