src/computational_monads/simulation_semantics/constructions/uniform_oracle.lean
@@ -1,0 +1,18 @@
+import computational_monads.simulation_semantics.constructions.stateless_oracle
+
+open oracle_comp oracle_spec
+
+variables {A B : Type} {spec spec' spec'' : oracle_spec}
+  (oa : oracle_comp spec A)
+
+noncomputable def uniform_oracle (spec : oracle_spec) [spec.finite_range] : 
+  simulation_oracle spec uniform_selecting :=
+⟪ λ i t, $ᵗ (spec.range i) ⟫
+
+@[simp]
+lemma default_state_uniform_oracle (spec : oracle_spec) [spec.finite_range] :
+  (uniform_oracle spec).default_state = () := rfl
+
+@[simp]
+lemma uniform_oracle_apply (spec : oracle_spec) (i : spec.ι) (t : spec.domain i) [spec.finite_range] (s : unit) :
+  (uniform_oracle spec).o i (t, s) = $ᵗ (spec.range i) >>= λ u, return (u, ()) := rfl
